Do Poly subst type/type again with split environments

proof/Poly/KiJudge.v
@@ -1,109 +1,46 @@
 
 Require Import Exp.
-Require Import TyEnv.
 Require Import WellFormed.
 Require Import Base.
 
 (* Kinds of types ***************************************************)
 
-Inductive KIND : tyenv -> ty -> ki -> Prop :=
+Inductive KIND : kienv -> ty -> ki -> Prop :=
  | KICon 
-   :  forall e c
-   ,  KIND e (TCon c) KStar
+   :  forall ke c
+   ,  KIND ke (TCon c) KStar
 
  | KIVar
-   :  forall e it k
-   ,  getK e it = Some (EKind k)
-   -> KIND e (TVar it) k
+   :  forall ke i k
+   ,  get  ke i = Some k
+   -> KIND ke (TVar i) k
 
  | KIForall
-   :  forall e t
-   ,  KIND (e :> EKind KStar) t          KStar
-   -> KIND e                 (TForall t) KStar
+   :  forall ke t
+   ,  KIND (ke :> KStar) t           KStar
+   -> KIND ke            (TForall t) KStar
 
  | KIFun 
-   :  forall e t1 t2
-   ,  KIND e t1 KStar -> KIND e t2 KStar
-   -> KIND e (TFun t1 t2) KStar.
+   :  forall ke t1 t2
+   ,  KIND ke t1 KStar
+   -> KIND ke t2 KStar
+   -> KIND ke (TFun t1 t2) KStar.
 Hint Constructors KIND.
 
 
 (* Well Formedness **************************************************)
-
 (* A well kinded type is well formed *)
 Lemma kind_wfT
- :  forall e t k
- ,  KIND e t k
- -> wfT  e t.
+ :  forall ke t k
+ ,  KIND ke t k
+ -> wfT  ke t.
 Proof.
- intros. gen e k.
+ intros. gen ke k.
  induction t; intros; inverts H; simpl; eauto.
 Qed.
 
 
-(* Weakening kind environment ***************************************)
-
-(* If we add a new kind to the environment of a well kinded type, 
-   then that type is still well kinded *)
-Lemma kind_weaken1
- :  forall e t1 k1 l
- ,  KIND e        t1 k1
- -> KIND (l <: e) t1 k1.
-Proof.
- intros. gen e k1.
- induction t1; intros; inverts H; eauto.
-
- Case "TVar".
-  apply KIVar. 
-  apply getMatch_cons_some. auto.
-
- Case "TForall".
-  apply KIForall.
-  rewrite snoc_cons. apply IHt1. auto.
-Qed.
-
-
-Lemma kind_weaken
- :  forall e1 e2 t1 k1
- ,  KIND e1         t1 k1
- -> KIND (e2 ++ e1) t1 k1.
-Proof.
- intros. gen e1 k1.
- induction e2; intros.
-  rewrite append_empty_left. auto.
-  rewrite append_snoc. apply IHe2.
-   apply kind_weaken1. auto.
-Qed.
-
-
-(* Strenghten kind environment **************************************)
-
-(* If a well kinded type doesn't use elements on the end of its
-   environment, then it is still well kinded if we cut them off *)
-Lemma kind_strengthen
- :  forall e e' n t k
- ,   wfT e' t
- ->  e' = take n e
- ->  KIND e  t k
- ->  KIND e' t k.
-Proof.
- intros. gen e e' n k.
- induction t; intros; inverts H1; eauto.
- Case "TVar".
-  apply KIVar. subst.
-  destruct H. admit. (* ok, list lemma *)
-
- Case "TForall".
-  apply KIForall. subst.
-  eapply IHt with (n := S n) (e := e :> EKind KStar); auto.
-
- Case "TFun".
-  simpl in H. destruct H. eauto. 
-Qed.
-
-
 (* Checking closed types ********************************************)
-
 (* If a type is well kinded in an empty environment,
    then that type is closed. *)
 Lemma kind_empty_is_closed
@@ -114,33 +51,4 @@ Proof.
  intros. unfold closedT. eapply kind_wfT. eauto.
 Qed.
 
-
-(* If a closed type is well kinded,
-   then it is well kinded in an empty environment. *)
-Lemma kind_closed_in_empty
- :  forall e t k
- ,  closedT t
- -> KIND e     t k
- -> KIND Empty t k.
-Proof.
- intros. unfold closedT in H.
- eapply kind_strengthen; eauto.
- eapply take_zero.
-Qed.
-
-
-(* If a closed type is well kinded,
-   then it is well kinded in an any environment. *)
-Theorem kind_closed_in_any
- :  forall e e' t k
- ,  closedT t
- -> KIND e  t k
- -> KIND e' t k.
-Proof.
- intros.
- lets D: kind_closed_in_empty H H0.
- assert (KIND (e' ++ Empty) t k).
-  apply kind_weaken. auto.
-  auto.
-Qed.
 
