proof/Poly/WellFormed.v
@@ -1,16 +1,15 @@
 
 Require Import Exp.
-Require Import TyEnv.
 
 
 (* Types ************************************************************)
 (* Well formed types are closed under the given kind environment *)
-Fixpoint wfT (e: tyenv) (tt: ty) : Prop := 
+Fixpoint wfT (ke: kienv) (tt: ty) : Prop := 
  match tt with
  | TCon _     => True
- | TVar i     => exists k, getK e i = Some k
- | TForall t  => wfT (e :> EKind KStar) t
- | TFun t1 t2 => wfT e t1 /\ wfT e t2
+ | TVar i     => exists k, get ke i = Some k
+ | TForall t  => wfT (ke :> KStar) t
+ | TFun t1 t2 => wfT ke t1 /\ wfT ke t2
  end.
 Hint Unfold wfT.
 
@@ -21,34 +20,22 @@ Definition closedT (tt: ty) : Prop
 Hint Unfold closedT.
 
 
-(* Environments ****************************************************)
-(* All types in a well formed environment are well formed under
-   the subsequent environment 
- *)
-Fixpoint wfEnv (e: tyenv) : Prop :=
- match e with 
- | Empty         => True
- | e' :> EKind _ => wfEnv e'
- | e' :> EType t => wfT e' t /\ wfEnv e'
- end.
-
-
 (* Expressions ******************************************************)
-(* A well formed expression is closed under the given environment *)
-Fixpoint wfX (e: tyenv) (xx: exp) : Prop := 
+(* A well formed expression is closed under the given environments *)
+Fixpoint wfX (ke: kienv) (te: tyenv) (xx: exp) : Prop := 
  match xx with 
- | XVar i     => exists t, getT e i = Some t
- | XLAM x     => wfX (e :> EKind KStar) x
- | XAPP x t   => wfX e x  /\ wfT e t
- | XLam t x   => wfT e t  /\ wfX (e :> EType t) x
- | XApp x1 x2 => wfX e x1 /\ wfX e x2
+ | XVar i     => exists t, get te i = Some t
+ | XLAM x     => wfX (ke :> KStar) te x
+ | XAPP x t   => wfX ke te x  /\ wfT ke t
+ | XLam t x   => wfT ke t     /\ wfX ke (te :> t) x
+ | XApp x1 x2 => wfX ke te x1 /\ wfX ke te x2
  end.
 Hint Unfold wfX.
 
 
 (* Closed expressions are well formed under empty environments *)
 Definition closedX (xx: exp) : Prop
- := wfX Empty xx.
+ := wfX Empty Empty xx.
 Hint Unfold closedX.
 
 
