proof/Poly/Exp.v
@@ -1,7 +1,13 @@
 
+Require Export Env.
+
+
 (* Kinds ************************************************************)
 Inductive ki : Type :=
  | KStar   : ki.
+
+Definition kienv := env ki.
+Hint Unfold kienv.
 
 
 (** Types ***********************************************************)
@@ -12,6 +18,9 @@ Inductive ty  : Type :=
  | TFun    : ty  -> ty -> ty.
 Hint Constructors ty.
 
+Definition tyenv := env ty.
+Hint Unfold tyenv.
+
 
 (** Expressions *****************************************************)
 Inductive exp : Type :=
@@ -21,4 +30,5 @@ Inductive exp : Type :=
  | XLam  : ty  -> exp -> exp
  | XApp  : exp -> exp -> exp.
 Hint Constructors exp.
+
 
